Finish update floyd/assert_lemmas.v

floyd/assert_lemmas.v
@@ -16,9 +16,9 @@ Proof. intros. destruct p; try contradiction; apply I. Qed.
 Hint Resolve isptr_offset_val': norm.
 
 Lemma sem_add_pi_ptr:
-   forall t p i, 
+   forall Delta t p i, 
     isptr p ->
-    sem_add_pi t p (Vint i) = Some (offset_val (Int.mul (Int.repr (sizeof t)) i) p).
+    sem_add_pi Delta t p (Vint i) = Some (offset_val (Int.mul (Int.repr (sizeof (composite_types Delta) t)) i) p).
 Proof. intros. destruct p; try contradiction. reflexivity. Qed.
 Hint Rewrite sem_add_pi_ptr using (solve [auto with norm]) : norm.
 
@@ -53,7 +53,7 @@ Proof.
 Qed.
 Hint Rewrite sem_cast_neutral_int using (solve [eauto with norm]) : norm.
 
-Lemma sizeof_tuchar: sizeof tuchar = 1%Z.
+Lemma sizeof_tuchar: forall cenv, sizeof cenv tuchar = 1%Z.
 Proof. reflexivity. Qed.
 Hint Rewrite sizeof_tuchar: norm.
 
@@ -196,24 +196,24 @@ Qed.
 Hint Rewrite overridePost_normal' : ret_assert.
 
 Lemma eval_expr_Etempvar: 
-  forall i t, eval_expr (Etempvar i t) = eval_id i.
+  forall Delta i t, eval_expr Delta (Etempvar i t) = eval_id i.
 Proof. reflexivity.
 Qed.
 Hint Rewrite eval_expr_Etempvar : eval.
 
-Lemma eval_expr_binop: forall op a1 a2 t, eval_expr (Ebinop op a1 a2 t) = 
-          `(eval_binop op (typeof a1) (typeof a2)) (eval_expr a1)  (eval_expr a2).
+Lemma eval_expr_binop: forall Delta op a1 a2 t, eval_expr Delta (Ebinop op a1 a2 t) = 
+          `(eval_binop Delta op (typeof a1) (typeof a2)) (eval_expr Delta a1) (eval_expr Delta a2).
 Proof. reflexivity. Qed.
 Hint Rewrite eval_expr_binop : eval.
 
-Lemma eval_expr_unop: forall op a1 t, eval_expr (Eunop op a1 t) = 
-          lift1 (eval_unop op (typeof a1)) (eval_expr a1).
+Lemma eval_expr_unop: forall Delta op a1 t, eval_expr Delta (Eunop op a1 t) = 
+          lift1 (eval_unop op (typeof a1)) (eval_expr Delta a1).
 Proof. reflexivity. Qed.
 Hint Rewrite eval_expr_unop : eval.
 
 Hint Resolve  eval_expr_Etempvar.
 
-Lemma eval_expr_Etempvar' : forall i t, eval_id i = eval_expr (Etempvar i t).
+Lemma eval_expr_Etempvar' : forall Delta i t, eval_id i = eval_expr Delta (Etempvar i t).
 Proof. intros. symmetry; auto.
 Qed.
 Hint Resolve  eval_expr_Etempvar'.
@@ -315,7 +315,7 @@ Qed.
 Hint Rewrite @subst_TT @subst_FF: subst.
 Hint Rewrite (@subst_TT mpred Nveric) (@subst_FF mpred Nveric): subst.
 
-Lemma eval_expr_Econst_int: forall i t, eval_expr (Econst_int i t) = `(Vint i).
+Lemma eval_expr_Econst_int: forall Delta i t, eval_expr Delta (Econst_int i t) = `(Vint i).
 Proof. reflexivity. Qed.
 Hint Rewrite eval_expr_Econst_int : eval.
 
@@ -333,7 +333,7 @@ Proof. reflexivity. Qed.
 Hint Rewrite subst_local : subst.
 
 Lemma eval_lvalue_Ederef:
-  forall e t, eval_lvalue (Ederef e t) = `force_ptr (eval_expr e).
+  forall Delta e t, eval_lvalue Delta (Ederef e t) = `force_ptr (eval_expr Delta e).
 Proof. reflexivity. Qed.
 Hint Rewrite eval_lvalue_Ederef : eval.
 
@@ -449,9 +449,9 @@ Proof. reflexivity. Qed.
 Hint Rewrite eval_make_args' : norm.
 
 Lemma eval_make_args_same:
- forall i t fsig t0 tl (e: expr) el,
- `(eval_id i) (make_args' ((i,t)::fsig, t0) (eval_exprlist (t::tl) (e::el))) = 
-   `force_val (`(sem_cast (typeof e) t) (eval_expr e)).
+ forall Delta i t fsig t0 tl (e: expr) el,
+ `(eval_id i) (make_args' ((i,t)::fsig, t0) (eval_exprlist Delta (t::tl) (e::el))) = 
+   `force_val (`(sem_cast (typeof e) t) (eval_expr Delta e)).
 Proof.
 intros.
 extensionality rho.
@@ -467,10 +467,10 @@ reflexivity.
 Qed.
 
 Lemma eval_make_args_other:
- forall i j fsig t0 t t' tl (e: expr) el,
+ forall Delta i j fsig t0 t t' tl (e: expr) el,
    i<>j ->
-  `(eval_id i) (make_args' ((j,t)::fsig, t0) (eval_exprlist (t'::tl) (e::el))) =
-   `(eval_id i) (make_args' (fsig, t0) (eval_exprlist tl el)).
+  `(eval_id i) (make_args' ((j,t)::fsig, t0) (eval_exprlist Delta (t'::tl) (e::el))) =
+   `(eval_id i) (make_args' (fsig, t0) (eval_exprlist Delta tl el)).
 Proof.
 intros. extensionality rho.
 unfold make_args'.
@@ -494,10 +494,10 @@ Proof. reflexivity. Qed.
 Hint Rewrite compose_backtick : norm.
 
 Lemma compose_eval_make_args_same:
-  forall (Q: val -> Prop) i t fsig t0 tl e el,
+  forall Delta (Q: val -> Prop) i t fsig t0 tl e el,
   @liftx (Tarrow environ (LiftEnviron Prop))
-      (Q oo (eval_id i)) (make_args' ((i,t)::fsig,t0) (eval_exprlist (t::tl) (e::el))) =
-  `Q (`force_val (`(sem_cast (typeof e) t) (eval_expr e))).
+      (Q oo (eval_id i)) (make_args' ((i,t)::fsig,t0) (eval_exprlist Delta (t::tl) (e::el))) =
+  `Q (`force_val (`(sem_cast (typeof e) t) (eval_expr Delta e))).
 Proof. 
   intros.
   rewrite <- compose_backtick.
@@ -505,11 +505,11 @@ Proof.
 Qed.
 
 Lemma compose_eval_make_args_other:
-  forall Q i j fsig t0 t t' tl (e: expr) el,
+  forall Delta Q i j fsig t0 t t' tl (e: expr) el,
    i<>j ->
     @liftx (Tarrow environ (LiftEnviron Prop))
-     (Q oo (eval_id i)) (make_args' ((j,t)::fsig, t0) (eval_exprlist (t'::tl) (e::el))) =
-     `Q (`(eval_id i) (make_args' (fsig, t0) (eval_exprlist tl el))).
+     (Q oo (eval_id i)) (make_args' ((j,t)::fsig, t0) (eval_exprlist Delta (t'::tl) (e::el))) =
+     `Q (`(eval_id i) (make_args' (fsig, t0) (eval_exprlist Delta tl el))).
 Proof.
   intros.
   rewrite <- compose_backtick.
@@ -561,9 +561,9 @@ Lemma elim_globals_only':
 Proof. reflexivity. Qed.
 Hint Rewrite elim_globals_only' : norm.
 
-Lemma eval_expropt_Some: forall e, eval_expropt (Some e) = `Some (eval_expr e).
+Lemma eval_expropt_Some: forall Delta e, eval_expropt Delta (Some e) = `Some (eval_expr Delta e).
 Proof. reflexivity. Qed.
-Lemma eval_expropt_None: eval_expropt None = `None.
+Lemma eval_expropt_None: forall Delta, eval_expropt Delta None = `None.
 Proof. reflexivity. Qed.
 Hint Rewrite eval_expropt_Some eval_expropt_None : eval.
 
@@ -1060,17 +1060,17 @@ Proof.
  left; split; omega. 
 Defined.
 
-Definition add_ptr_int' (ty: type) (v: val) (i: Z) : val :=
-  if repable_signed_dec (sizeof ty * i)
+Definition add_ptr_int' Delta (ty: type) (v: val) (i: Z) : val :=
+  if repable_signed_dec (sizeof (composite_types Delta) ty * i)
    then match v with
       | Vptr b ofs => 
-           Vptr b (Int.add ofs (Int.repr (sizeof ty * i)))
+           Vptr b (Int.add ofs (Int.repr (sizeof (composite_types Delta) ty * i)))
       | _ => Vundef
       end
   else Vundef.
 
-Definition add_ptr_int (ty: type) (v: val) (i: Z) : val :=
-           eval_binop Oadd (tptr ty) tint v (Vint (Int.repr i)).
+Definition add_ptr_int Delta (ty: type) (v: val) (i: Z) : val :=
+           eval_binop Delta Oadd (tptr ty) tint v (Vint (Int.repr i)).
 
 Lemma repable_signed_mult2:
   forall i j, i<>0 -> (j <= Int.max_signed \/ i <> -1) ->
@@ -1127,9 +1127,9 @@ intros.
 Qed.
 
 Lemma add_ptr_int_eq:
-  forall ty v i, 
-       repable_signed (sizeof ty * i) ->
-       add_ptr_int' ty v i = add_ptr_int ty v i.
+  forall Delta ty v i, 
+       repable_signed (sizeof (composite_types Delta) ty * i) ->
+       add_ptr_int' Delta ty v i = add_ptr_int Delta ty v i.
 Proof.
  intros.
  unfold add_ptr_int, add_ptr_int'.
@@ -1139,10 +1139,10 @@ Proof.
 Qed.
 
 Lemma add_ptr_int_offset:
-  forall t v n, 
-  repable_signed (sizeof t) ->
+  forall Delta t v n, 
+  repable_signed (sizeof (composite_types Delta) t) ->
   repable_signed n ->
-  add_ptr_int t v n = offset_val (Int.repr (sizeof t * n)) v.
+  add_ptr_int Delta t v n = offset_val (Int.repr (sizeof (composite_types Delta) t * n)) v.
 Proof.
  unfold add_ptr_int; intros.
  unfold eval_binop, force_val2; destruct v; simpl; auto.
@@ -1153,9 +1153,9 @@ Proof.
 Qed.
 
 Lemma add_ptr_int'_offset:
-  forall t v n, 
-  repable_signed (sizeof t * n) ->
-  add_ptr_int' t v n = offset_val (Int.repr (sizeof t * n)) v.
+  forall Delta t v n, 
+  repable_signed (sizeof (composite_types Delta) t * n) ->
+  add_ptr_int' Delta t v n = offset_val (Int.repr (sizeof (composite_types Delta) t * n)) v.
 Proof.
  intros.
  unfold add_ptr_int'. 
